@prefix customer: <http://bibsysdev.github.io/src/customer-ontology#> .
@prefix rdf: <http://www.w3.org/1999/02/22-rdf-syntax-ns#> .
@prefix rdfs: <http://www.w3.org/2000/01/rdf-schema#> .
@prefix xsd: <http://www.w3.org/2001/XMLSchema#> .
@prefix dcterms: <http://purl.org/dc/terms/> .
@prefix nva: <https://example.org/todo#> .

customer:VocabularySetting a rdfs:Class ;
  rdf:label "VocabularySetting" ;
  rdfs:comment "A set of customer-defined options defining the allowed usage of a controlled vocabulary" ;
  rdfs:isDefinedBy customer: .

customer:Disabled a rdfs:Class ;
  rdf:label "Disabled" ;
  rdfs:comment "A value denoting that a controlled vocabulary is not to be used" ;
  rdfs:isDefinedBy customer: ;
  rdfs:subClassOf customer:VocabularySettings .

customer:Allowed a rdfs:Class ;
  rdf:label "Allowed" ;
  rdfs:comment "A value denoting that a controlled vocabulary may be used" ;
  rdfs:isDefinedBy customer: ;
  rdfs:subClassOf customer:VocabularySettings .

customer:Default a rdfs:Class ;
  rdf:label "Default" ;
  rdfs:comment "A value denoting that a controlled vocabulary may be used and should be displayed by default" ;
  rdfs:isDefinedBy customer: ;
  rdfs:subClassOf customer:Allowed .

customer:legalName a rdf:Property ;
  rdf:label "legalName" ;
  rdfs:comment "A literal string by which an institution is known in official registers" ;
  rdfs:isDefinedBy customer: ;
  rdfs:isSubPropertyOf rdfs:label ;
  rdfs:domain nva:Organization ;
  rdfs:range xsd:string .

customer:displayName a rdf:Property ;
  rdf:label "displayName" ;
  rdfs:comment "A literal string to be used when presenting an institution as text to users" ;
  rdfs:isDefinedBy customer: ;
  rdfs:isSubPropertyOf rdfs:label ;
  rdfs:domain nva:Organization ;
  rdfs:range xsd:string .

customer:shortName a rdf:Property ;
  rdf:label "shortName" ;
  rdfs:comment "An abbreviation of an institution name" ;
  rdfs:isDefinedBy customer: ;
  rdfs:isSubPropertyOf rdfs:label ;
  rdfs:domain nva:Organization ;
  rdfs:range xsd:string .

customer:archiveName a rdf:Property ;
  rdf:label "archiveName" ;
  rdfs:comment "A name used when describing the set of data owned by an institution" ;
  rdfs:isDefinedBy customer: ;
  rdfs:isSubPropertyOf rdfs:label ;
  rdfs:domain nva:Organization ;
  rdfs:range xsd:string .

customer:cname a rdf:Property ;
  rdf:label "cname" ;
  rdfs:comment "A Canonical Name (DNS) that should resolve the set of data owned by an institution" ;
  rdfs:isDefinedBy customer: ;
  rdfs:domain nva:Organization ;
  rdfs:range xsd:string .

customer:institutionDns a rdf:Property ;
  rdf:label "institutionDns" ;
  rdfs:comment "A Domain Name System used by an institution" ;
  rdfs:isDefinedBy customer: ;
  rdfs:domain nva:Organization ;
  rdfs:range xsd:string .

customer:feideOrganizationId a rdf:Property ;
  rdf:label "feideOrganizationId" ;
  rdfs:comment "A Feide organization ID of an institution" ;
  rdfs:isDefinedBy customer: ;
  rdfs:domain nva:Organization ;
  rdfs:range xsd:string .

customer:cristinId a rdf:Property ;
  rdf:label "cristinId" ;
  rdfs:comment "An identifier in the Cristin organization register associated with an institution" ;
  rdfs:isDefinedBy customer: ;
  rdfs:domain nva:Organization ;
  rdfs:range xsd:string .

customer:vocabularySetting a rdf:Property ;
  rdf:label "vocabularySetting" ;
  rdfs:comment "A resource defining the usage of a controlled vocabulary" ;
  rdfs:isDefinedBy customer: ;
  rdfs:domain nva:Organization ;
  rdfs:range customer:VocabularySetting .

customer:vocabularyUsage a rdf:Property ;
  rdf:label "vocabularyUsage" ;
  rdfs:comment "A definition of the allowed usage of a controlled vocabulary" ;
  rdfs:isDefinedBy customer: ;
  rdfs:domain customer:VocabularySetting ;
  rdfs:range customer:VocabularyStatus .